src/interfaces/orders.v
@@ -1,0 +1,24 @@
+Require Import abstract_algebra.
+
+
+Class PartialOrder `{Ae : Equiv A} (Ale : Le A) (P:Subset A) : Prop :=
+  { po_subsetoid : SubSetoid P
+  ; po_proper  : Proper ((P,=) ==> (P,=) ==> impl) (≤)
+  ; po_refl    :> SubReflexive  (≤) P
+  ; po_trans   :> SubTransitive (≤) P
+  ; po_antisym :> SubAntiSymmetric (≤) P
+  }.
+
+Class TotalOrder `{Ae : Equiv A} (Ale : Le A) (S:Subset A) : Prop :=
+  { total_order_po :> PartialOrder (≤) S
+  ; total_order_total :> TotalRelation (≤) S
+  }.
+
+Class SubStrictOrder `{Ae : Equiv A} (Alt : Lt A) (S:Subset A) : Prop :=
+  { so_subsetoid : SubSetoid S
+  ; so_proper  : Proper ((S,=) ==> (S,=) ==> impl) (<)
+  ; so_irrefl  :> SubIrreflexive (<) S
+  ; so_trans   :> SubTransitive  (<) S
+  }.
+
+
